* Simplifying the language to just logic and arithmetic so simple versions of all the proofs can be constructed.  Will then go back and add variables and functions and extend the proofs. * Proof of determinism of Typing for the simplified surface syntax * Minor tweaks

Total/Stlc/Lang/Surface/Grammar.lean
@@ -1,10 +1,8 @@
 namespace Total.Stlc.Lang.Surface
-  mutual
-    inductive Ty: Type where
-      | bool: Ty
-      | nat: Ty
-      -- | fn (dom: List Ty) (rng: Ty): Ty
-  end
+  inductive Ty: Type where
+    | bool: Ty
+    | nat: Ty
+    -- | fn (dom: List Ty) (rng: Ty): Ty
 
   inductive Term: Type where
     | bool (b: Bool): Term
@@ -13,7 +11,6 @@ namespace Total.Stlc.Lang.Surface
     | or (lhs rhs: Term): Term
     | not (op: Term): Term
     | add (lhs rhs: Term): Term
-    | sub (lhs rhs: Term): Term
     | mul (lhs rhs: Term): Term
     | eq (lhs rhs: Term): Term
     | neq (lhs rhs: Term): Term
