Total/Stlc/Lang/Surface/Theorems.lean
@@ -10,17 +10,43 @@ namespace Total.Stlc.Lang.Surface
 
   namespace Term
     namespace HasType
-      theorem deterministic {ε: Env} {t: Term} {τ₁ τ₂: Ty}: HasType ε t τ₁ → HasType ε t τ₂ → τ₁ = τ₂ := sorry
+      theorem deterministic {t: Term} {τ₁ τ₂: Ty}: HasType t τ₁ → HasType t τ₂ → τ₁ = τ₂
+        | .bool, .bool
+        | .nat,  .nat  => rfl
+
+        | .and _ _, .and _ _
+        | .or  _ _, .or  _ _
+        | .not _,   .not _   => rfl
+
+        | .add _ _, .add _ _
+        | .mul _ _, .mul _ _ => rfl
+
+        | .eq  _ _, .eq  _ _
+        | .neq _ _, .neq _ _ => rfl
+
+        | .lt  _ _, .lt  _ _
+        | .lte _ _, .lte _ _
+        | .gt  _ _, .gt  _ _
+        | .gte _ _, .gte _ _ => rfl
+
+        | .cond _ t₁ _, .cond _ t₂ _ =>
+          have ih₂ := deterministic t₁ t₂
+          by rw [ih₂]
+
+        | .lt  _ _, .gt  _ _
+        | .lte _ _, .gte _ _
+        | .gt  _ _, .lt  _ _
+        | .gte _ _, .lte _ _ => rfl
     end HasType
 
     namespace Eval₁
       theorem deterministic {t t₁ t₂: Term}: Eval₁ t t₁ → Eval₁ t t₂ → t₁ = t₂ := sorry
-      theorem preservation {ε: Env} {τ: Ty} {t₁ t₂: Term}: HasType ε t₁ τ → Eval₁ t₁ t₂ → HasType ε t₂ τ := sorry
-      theorem progress {ε: Env} {τ: Ty} {t₁: Term}: HasType ε t₁ τ → IsValue t₁ ∨ ∃ t₂: Term, Eval₁ t₁ t₂ := sorry
+      theorem preservation {τ: Ty} {t₁ t₂: Term}: HasType t₁ τ → Eval₁ t₁ t₂ → HasType t₂ τ := sorry
+      theorem progress {τ: Ty} {t₁: Term}: HasType t₁ τ → IsValue t₁ ∨ ∃ t₂: Term, Eval₁ t₁ t₂ := sorry
 
       -- TODO: Theorems for Strong Normalization
-      theorem confluent {ε: Env} {τ: Ty} {t₁ t₂ t₃: Term}: Eval₁ t₁ t₂ → Eval₁ t₁ t₃ → ∃ t₄: Term, Eval₁ t₂ t₄ ∧ Eval₁ t₃ t₄ := sorry
-      theorem strongly_normalizing {ε: Env} {τ: Ty} {t₁: Term}: IsValue t₁ ∨ ∃ t₂: Term, Eval₁ t₁ t₂ := sorry
+      theorem confluent {τ: Ty} {t₁ t₂ t₃: Term}: Eval₁ t₁ t₂ → Eval₁ t₁ t₃ → ∃ t₄: Term, Eval₁ t₂ t₄ ∧ Eval₁ t₃ t₄ := sorry
+      theorem strongly_normalizing {τ: Ty} {t₁: Term}: IsValue t₁ ∨ ∃ t₂: Term, Eval₁ t₁ t₂ := sorry
     end Eval₁
   end Term
 
